Spec structure filled out to create core obligations. Spec has async operations and crash tolerance

Splinter/IOSystem.s.dfy
@@ -1,80 +1,365 @@
+// Copyright 2018-2021 VMware, Inc., Microsoft Inc., Carnegie Mellon University, ETH Zurich, and University of Washington
+// SPDX-License-Identifier: BSD-2-Clause
+
+include "Spec.s.dfy"
+include "../lib/Base/MapRemove.s.dfy"
+include "../lib/Checksums/CRC32C.s.dfy"
 include "Allocation.i.dfy"
 include "StateMachine.s.dfy"
-include "Spec.s.dfy"
 
-module Disk {
-  import opened AllocationMod
-  datatype Variables = Variables(dv: DiskView)
+//
+// An async disk allows concurrent outstanding I/Os. The disk is a sequence of bytes.
+//
+// (Real disks constrain I/Os to fall on logical-block-address boundaries, but we're
+// ignoring constraint for now.)
+//
 
-  predicate Init(v: Variables)
-  {
-    true  // TODO fill in
-  }
-}
+module AsyncDisk {
+  import opened NativeTypes
+  import opened MapRemove_s
+  import CRC32_C
 
-abstract module IOSystem {
-  import Disk
-  import ProgramParam : StateMachine // abstract import -- to be filled in by final theorem
+  type ReqId = uint64
+
+  datatype ReqRead = ReqRead(addr: uint64, len: uint64)
+  datatype ReqWrite = ReqWrite(addr: uint64, bytes: seq<byte>)
+  datatype RespRead = RespRead(addr: uint64, bytes: seq<byte>)
+  datatype RespWrite = RespWrite(addr: uint64, len: uint64)
+
+  datatype DiskOp =
+    | ReqReadOp(id: ReqId, reqRead: ReqRead)
+    | ReqWriteOp(id: ReqId, reqWrite: ReqWrite)
+    | ReqWrite2Op(id1: ReqId, id2: ReqId,
+        reqWrite1: ReqWrite, reqWrite2: ReqWrite)
+    | RespReadOp(id: ReqId, respRead: RespRead)
+    | RespWriteOp(id: ReqId, respWrite: RespWrite)
+    | NoDiskOp
 
   datatype Variables = Variables(
-    program: ProgramParam.Variables,
-    disk: Disk.Variables)
+    // Queue of requests and responses:
+    reqReads: map<ReqId, ReqRead>,
+    reqWrites: map<ReqId, ReqWrite>,
+    respReads: map<ReqId, RespRead>,
+    respWrites: map<ReqId, RespWrite>,
 
-  predicate Init(v: Variables)
+    // The disk:
+    contents: seq<byte>
+  )
+
+  predicate Init(s: Variables)
   {
-    && Disk.Mkfs(v.disk)
-    && ProgramParam.Init(v.program)
+    && s.reqReads == map[]
+    && s.reqWrites == map[]
+    && s.respReads == map[]
+    && s.respWrites == map[]
   }
 
-  predicate Crash(v: Variables, v': Variables)
+  datatype Step =
+    | RecvReadStep
+    | RecvWriteStep
+    | RecvWrite2Step
+    | AckReadStep
+    | AckWriteStep
+    | StutterStep
+
+  predicate RecvRead(s: Variables, s': Variables, dop: DiskOp)
   {
-    && v'.disk == v.disk
-    // TODO cancel in-flight I/Os -- when we add disk asynchrony
-    && ProgramParam.Init(v.program)
+    && dop.ReqReadOp?
+    && dop.id !in s.reqReads
+    && dop.id !in s.respReads
+    && s' == s.(reqReads := s.reqReads[dop.id := dop.reqRead])
   }
 
-  predicate Normal(v: Variables, v': Variables, diskOps: DiskOps)
+  predicate RecvWrite(s: Variables, s': Variables, dop: DiskOp)
   {
-    && Disk.Next(v, v', diskOps)
-    && ProgramParam.Next(v, v', diskOps)
+    && dop.ReqWriteOp?
+    && dop.id !in s.reqWrites
+    && dop.id !in s.respWrites
+    && s' == s.(reqWrites := s.reqWrites[dop.id := dop.reqWrite])
   }
 
-  datatype Step = CrashStep | NormalStep(diskOps: DiskOps)
-
-  predicate NextStep(v: Variables, v': Variables, step: Step)
+  predicate RecvWrite2(s: Variables, s': Variables, dop: DiskOp)
   {
+    && dop.ReqWrite2Op?
+    && dop.id1 !in s.reqWrites
+    && dop.id1 !in s.respWrites
+    && dop.id2 !in s.reqWrites
+    && dop.id2 !in s.respWrites
+    && dop.id1 != dop.id2
+    && s' == s.(reqWrites :=
+        s.reqWrites[dop.id1 := dop.reqWrite1]
+                   [dop.id2 := dop.reqWrite2]
+       )
+  }
+
+  predicate AckRead(s: Variables, s': Variables, dop: DiskOp)
+  {
+    && dop.RespReadOp?
+    && dop.id in s.respReads
+    && s.respReads[dop.id] == dop.respRead
+    && s' == s.(respReads := MapRemove1(s.respReads, dop.id))
+  }
+
+  predicate AckWrite(s: Variables, s': Variables, dop: DiskOp)
+  {
+    && dop.RespWriteOp?
+    && dop.id in s.respWrites
+    && s.respWrites[dop.id] == dop.respWrite
+    && s' == s.(respWrites := MapRemove1(s.respWrites, dop.id))
+  }
+
+  predicate Stutter(s: Variables, s': Variables, dop: DiskOp)
+  {
+    && dop.NoDiskOp?
+    && s' == s
+  }
+
+  predicate NextStep(s: Variables, s': Variables, dop: DiskOp, step: Step) {
     match step {
-      CrashStep => Crash(v, v')
-      NormalStep(diskOps) => Normal(v, v', diskOps)
+      case RecvReadStep => RecvRead(s, s', dop)
+      case RecvWriteStep => RecvWrite(s, s', dop)
+      case RecvWrite2Step => RecvWrite2(s, s', dop)
+      case AckReadStep => AckRead(s, s', dop)
+      case AckWriteStep => AckWrite(s, s', dop)
+      case StutterStep => Stutter(s, s', dop)
     }
   }
 
-  predicate Next(v: Variables, v': Variables)
+  predicate Next(s: Variables, s': Variables, dop: DiskOp) {
+    exists step :: NextStep(s, s', dop, step)
+  }
+
+  datatype InternalStep =
+    //| ProcessReadStep(id: ReqId)
+    | ProcessReadFailureStep(id: ReqId, fakeContents: seq<byte>)
+    | ProcessWriteStep(id: ReqId)
+    | HavocConflictingWritesStep(id: ReqId, id': ReqId)
+    | HavocConflictingWriteReadStep(id: ReqId, id': ReqId)
+
+  /*predicate ProcessRead(s: Variables, s': Variables, id: ReqId)
   {
-    exists step :: NextStep(v, v', step)
+    && id in s.reqReads
+    && var req := s.reqReads[id];
+    && 0 <= req.addr as int <= req.addr as int + req.len as int <= |s.contents|
+    && s' == s.(reqReads := MapRemove1(s.reqReads, id))
+              .(respReads := s.respReads[id := RespRead(req.addr, s.contents[req.addr .. req.addr as int + req.len as int])])
+  }*/
+
+  predicate {:opaque} ChecksumChecksOut(s: seq<byte>) {
+    && |s| >= 32
+    && s[0..32] == CRC32_C.crc32_c_padded(s[32..])
+  }
+
+  predicate ChecksumsCheckOutForSlice(realContents: seq<byte>, fakeContents: seq<byte>, i: int, j: int)
+  requires |realContents| == |fakeContents|
+  requires 0 <= i <= j <= |realContents|
+  {
+    // We make the assumption that the disk cannot fail from a checksum-correct state
+    // to a different checksum-correct state. This is a reasonable assumption for many
+    // probabilistic failure models of the disk.
+
+    // We don't make a blanket assumption that !ChecksumChecksOut(fakeContents)
+    // because it would be reasonable for a disk to fail into a checksum-correct state
+    // from a checksum-incorrect one.
+
+    ChecksumChecksOut(realContents[i..j]) && 
+    ChecksumChecksOut(fakeContents[i..j]) ==>
+        realContents[i..j] == fakeContents[i..j]
+  }
+
+  predicate AllChecksumsCheckOut(realContents: seq<byte>, fakeContents: seq<byte>)
+  requires |realContents| == |fakeContents|
+  {
+    forall i, j | 0 <= i <= j <= |realContents| ::
+      ChecksumsCheckOutForSlice(realContents, fakeContents, i, j)
+  }
+
+  predicate ProcessReadFailure(s: Variables, s': Variables, id: ReqId, fakeContents: seq<byte>)
+  {
+    && id in s.reqReads
+    && var req := s.reqReads[id];
+    && 0 <= req.addr as int <= req.addr as int + req.len as int <= |s.contents|
+    && var realContents := s.contents[req.addr .. req.addr as int + req.len as int];
+    && |fakeContents| == |realContents|
+    && fakeContents != realContents
+
+    && AllChecksumsCheckOut(realContents, fakeContents)
+
+    && s' == s.(reqReads := MapRemove1(s.reqReads, id))
+              .(respReads := s.respReads[id := RespRead(req.addr, fakeContents)])
+  }
+
+  function {:opaque} splice(bytes: seq<byte>, start: int, ins: seq<byte>) : seq<byte>
+  requires 0 <= start
+  requires start + |ins| <= |bytes|
+  {
+    bytes[.. start] + ins + bytes[start + |ins| ..]
+  }
+
+  predicate ProcessWrite(s: Variables, s': Variables, id: ReqId)
+  {
+    && id in s.reqWrites
+    && var req := s.reqWrites[id];
+    && 0 <= req.addr
+    && |req.bytes| < 0x1_0000_0000_0000_0000
+    && req.addr as int + |req.bytes| <= |s.contents|
+    && s' == s.(reqWrites := MapRemove1(s.reqWrites, id))
+              .(respWrites := s.respWrites[id := RespWrite(req.addr, |req.bytes| as uint64)])
+              .(contents := splice(s.contents, req.addr as int, req.bytes))
+  }
+
+  // We assume the disk makes ABSOLUTELY NO GUARANTEES about what happens
+  // when there are conflicting reads or writes.
+
+  predicate overlap(start: int, len: int, start': int, len': int)
+  {
+    && start + len > start'
+    && start' + len' > start
+  }
+
+  predicate HavocConflictingWrites(s: Variables, s': Variables, id: ReqId, id': ReqId)
+  {
+    && id != id'
+    && id in s.reqWrites
+    && id' in s.reqWrites
+    && overlap(
+        s.reqWrites[id].addr as int, |s.reqWrites[id].bytes|,
+        s.reqWrites[id'].addr as int, |s.reqWrites[id'].bytes|)
+  }
+
+  predicate HavocConflictingWriteRead(s: Variables, s': Variables, id: ReqId, id': ReqId)
+  {
+    && id in s.reqWrites
+    && id' in s.reqReads
+    && overlap(
+        s.reqWrites[id].addr as int, |s.reqWrites[id].bytes|,
+        s.reqReads[id'].addr as int, s.reqReads[id'].len as int)
+  }
+
+  predicate NextInternalStep(s: Variables, s': Variables, step: InternalStep)
+  {
+    match step {
+      //case ProcessReadStep(id) => ProcessRead(s, s', id)
+      case ProcessReadFailureStep(id, fakeContents) => ProcessReadFailure(s, s', id, fakeContents)
+      case ProcessWriteStep(id) => ProcessWrite(s, s', id)
+      case HavocConflictingWritesStep(id, id') => HavocConflictingWrites(s, s', id, id')
+      case HavocConflictingWriteReadStep(id, id') => HavocConflictingWriteRead(s, s', id, id')
+    }
+  }
+
+  predicate NextInternal(s: Variables, s': Variables)
+  {
+    exists step :: NextInternalStep(s, s', step)
+  }
+
+  predicate Crash(s: Variables, s': Variables)
+  {
+    s' == Variables(map[], map[], map[], map[], s.contents)
+  }
+}
+
+// Interface to the implementer-supplied program that is getting verified.
+abstract module AsyncDiskProgram {
+  import D = AsyncDisk  // Importing for the interface, not the entire disk
+  import CrashTolerantMapSpecMod
+
+  type Variables
+  type UIOp = CrashTolerantMapSpecMod.UIOp
+
+  type DiskOp = D.DiskOp
+  type ReqRead = D.ReqRead
+  type ReqWrite = D.ReqWrite
+  type RespRead = D.RespRead
+  type RespWrite = D.RespWrite
+
+  predicate Init(s: Variables)
+  predicate Next(s: Variables, s': Variables, uiop: UIOp, dop: DiskOp)
+}
+
+abstract module IOSystem {
+  import D = AsyncDisk
+  import P : AsyncDiskProgram
+  import opened NativeTypes
+
+  type DiskOp = P.DiskOp
+  datatype Variables = Variables(program: P.Variables, disk: D.Variables)
+  type UIOp = P.UIOp
+
+  datatype Step =
+    | MachineStep(dop: DiskOp)
+    | DiskInternalStep(step: D.InternalStep)
+    | CrashStep
+  
+  predicate Machine(s: Variables, s': Variables, uiop: UIOp, dop: DiskOp)
+  {
+    && P.Next(s.program, s'.program, uiop, dop)
+    && D.Next(s.disk, s'.disk, dop)
+  }
+
+  predicate DiskInternal(s: Variables, s': Variables, uiop: UIOp, step: D.InternalStep)
+  {
+    && uiop.NoopOp?
+    && s.program == s'.program
+    && D.NextInternalStep(s.disk, s'.disk, step)
+  }
+
+  predicate Crash(s: Variables, s': Variables, uiop: UIOp)
+  {
+    && uiop.CrashOp?
+    && P.Init(s'.program)
+    && D.Crash(s.disk, s'.disk)
+  }
+
+  predicate NextStep(s: Variables, s': Variables, uiop: UIOp, step: Step)
+  {
+    match step {
+      case MachineStep(dop) => Machine(s, s', uiop, dop)
+      case DiskInternalStep(step) => DiskInternal(s, s', uiop, step)
+      case CrashStep => Crash(s, s', uiop)
+    }
+  }
+
+  predicate Next(s: Variables, s': Variables, uiop: UIOp) {
+    exists step :: NextStep(s, s', uiop, step)
+  }
+
+  predicate BlocksWrittenInByteSeq(
+      contents: map<uint64, seq<byte>>,
+      byteSeq: seq<byte>)
+  {
+    && (forall addr: uint64 | addr in contents ::
+        && 0 <= addr as int <= |byteSeq|
+        && addr as int + |contents[addr]| <= |byteSeq|
+        && byteSeq[addr .. addr as int + |contents[addr]|] == contents[addr])
+  }
+
+  predicate BlocksDontIntersect(contents: map<uint64, seq<byte>>)
+  {
+    && (forall addr1, addr2 | addr1 in contents && addr2 in contents
+        && addr1 != addr2 :: !D.overlap(addr1 as int, |contents[addr1]|, addr2 as int, |contents[addr2]|))
   }
 }
 
 abstract module ProofObligations {
-  import DeferredWriteMapSpecMod
+  import CrashTolerantMapSpecMod
   import ConcreteSystem : IOSystem
 
   // Your interpretation function
-  function I(v: ConcreteSystem.Variables) : DeferredWriteMapSpecMod.Variables
+  function I(v: ConcreteSystem.Variables) : CrashTolerantMapSpecMod.Variables
 
   // Your system invariant
   predicate Inv(v: ConcreteSystem.Variables)
 
   lemma InitRefines(v: ConcreteSystem.Variables)
-    ensures DeferredWriteMapSpecMod.Init(I(v))
+    ensures CrashTolerantMapSpecMod.Init(I(v))
 
-  lemma InvInductive(v: ConcreteSystem.Variables, v': ConcreteSystem.Variables)
+  lemma InvInductive(v: ConcreteSystem.Variables, v': ConcreteSystem.Variables, uiop: ConcreteSystem.UIOp)
     requires Inv(v)
-    requires ConcreteSystem.Next(v, v')
+    requires ConcreteSystem.Next(v, v', uiop)
     ensures Inv(v')
 
-  lemma NextRefines(v: ConcreteSystem.Variables, v': ConcreteSystem.Variables)
+  lemma NextRefines(v: ConcreteSystem.Variables, v': ConcreteSystem.Variables, uiop: ConcreteSystem.UIOp)
     requires Inv(v)
-    requires ConcreteSystem.Next(v, v')
-    ensures DeferredWriteMapSpecMod.Next(I(v), I(v'))
+    requires ConcreteSystem.Next(v, v', uiop)
+    ensures CrashTolerantMapSpecMod.Next(I(v), I(v'), uiop)
 }
